Aux.ec
@@ -3,3 +3,29 @@ require import AllCore.
 lemma andI (a b : bool) : a => b => a /\ b.
 auto.
 qed.
+
+
+lemma oip1 (a b c eps : real) :  (0%r <= eps) =>
+  `|a / b - c| <= eps
+ => exists (p : real), 0%r <= p <= eps  /\ `|a / b - c| = p.
+smt.
+qed.
+
+
+lemma oip2 (a b c p : real) :  
+  (0%r < b) =>
+  `|a / b - c| = p =>
+      a = b * c - b * p \/  a = b * c + b * p.
+smt.
+qed.
+
+
+
+lemma oip3 (a b c eps : real) :  (0%r < b) => (0%r <= eps) =>
+  `|a / b - c| <= eps => 
+  exists (p : real),  0%r <= p <= eps  
+  /\ `|a / b - c| = p 
+  /\ (a = b * (c - p) \/  a = b * (c + p)).
+smt (oip1 oip2).
+qed.
+
